theories/AutoSubst/Ast.v
@@ -18,7 +18,7 @@ Inductive term : Type :=
   | tEmpty : term
   | tEmptyElim : term -> term -> term
   | tSig : term -> term -> term
-  | tPair : term -> term -> term -> term -> term
+  | tPair : option (term) -> term -> term -> term
   | tFst : term -> term
   | tSnd : term -> term.
 
@@ -98,16 +98,14 @@ exact (eq_trans (eq_trans eq_refl (ap (fun x => tSig x s1) H0))
          (ap (fun x => tSig t0 x) H1)).
 Qed.
 
-Lemma congr_tPair {s0 : term} {s1 : term} {s2 : term} {s3 : term} {t0 : term}
-  {t1 : term} {t2 : term} {t3 : term} (H0 : s0 = t0) (H1 : s1 = t1)
-  (H2 : s2 = t2) (H3 : s3 = t3) : tPair s0 s1 s2 s3 = tPair t0 t1 t2 t3.
+Lemma congr_tPair {s0 : option (term)} {s1 : term} {s2 : term}
+  {t0 : option (term)} {t1 : term} {t2 : term} (H0 : s0 = t0) (H1 : s1 = t1)
+  (H2 : s2 = t2) : tPair s0 s1 s2 = tPair t0 t1 t2.
 Proof.
 exact (eq_trans
-         (eq_trans
-            (eq_trans (eq_trans eq_refl (ap (fun x => tPair x s1 s2 s3) H0))
-               (ap (fun x => tPair t0 x s2 s3) H1))
-            (ap (fun x => tPair t0 t1 x s3) H2))
-         (ap (fun x => tPair t0 t1 t2 x) H3)).
+         (eq_trans (eq_trans eq_refl (ap (fun x => tPair x s1 s2) H0))
+            (ap (fun x => tPair t0 x s2) H1))
+         (ap (fun x => tPair t0 t1 x) H2)).
 Qed.
 
 Lemma congr_tFst {s0 : term} {t0 : term} (H0 : s0 = t0) : tFst s0 = tFst t0.
@@ -147,9 +145,9 @@ Fixpoint ren_term (xi_term : nat -> nat) (s : term) {struct s} : term :=
         (ren_term xi_term s1)
   | tSig s0 s1 =>
       tSig (ren_term xi_term s0) (ren_term (upRen_term_term xi_term) s1)
-  | tPair s0 s1 s2 s3 =>
-      tPair (ren_term xi_term s0) (ren_term (upRen_term_term xi_term) s1)
-        (ren_term xi_term s2) (ren_term xi_term s3)
+  | tPair s0 s1 s2 =>
+      tPair (option_map (ren_term (upRen_term_term xi_term)) s0)
+        (ren_term xi_term s1) (ren_term xi_term s2)
   | tFst s0 => tFst (ren_term xi_term s0)
   | tSnd s0 => tSnd (ren_term xi_term s0)
   end.
@@ -185,10 +183,9 @@ term :=
   | tSig s0 s1 =>
       tSig (subst_term sigma_term s0)
         (subst_term (up_term_term sigma_term) s1)
-  | tPair s0 s1 s2 s3 =>
-      tPair (subst_term sigma_term s0)
-        (subst_term (up_term_term sigma_term) s1) (subst_term sigma_term s2)
-        (subst_term sigma_term s3)
+  | tPair s0 s1 s2 =>
+      tPair (option_map (subst_term (up_term_term sigma_term)) s0)
+        (subst_term sigma_term s1) (subst_term sigma_term s2)
   | tFst s0 => tFst (subst_term sigma_term s0)
   | tSnd s0 => tSnd (subst_term sigma_term s0)
   end.
@@ -235,11 +232,12 @@ subst_term sigma_term s = s :=
   | tSig s0 s1 =>
       congr_tSig (idSubst_term sigma_term Eq_term s0)
         (idSubst_term (up_term_term sigma_term) (upId_term_term _ Eq_term) s1)
-  | tPair s0 s1 s2 s3 =>
-      congr_tPair (idSubst_term sigma_term Eq_term s0)
-        (idSubst_term (up_term_term sigma_term) (upId_term_term _ Eq_term) s1)
+  | tPair s0 s1 s2 =>
+      congr_tPair
+        (option_id
+           (idSubst_term (up_term_term sigma_term) (upId_term_term _ Eq_term))
+           s0) (idSubst_term sigma_term Eq_term s1)
         (idSubst_term sigma_term Eq_term s2)
-        (idSubst_term sigma_term Eq_term s3)
   | tFst s0 => congr_tFst (idSubst_term sigma_term Eq_term s0)
   | tSnd s0 => congr_tSnd (idSubst_term sigma_term Eq_term s0)
   end.
@@ -291,12 +289,13 @@ ren_term xi_term s = ren_term zeta_term s :=
       congr_tSig (extRen_term xi_term zeta_term Eq_term s0)
         (extRen_term (upRen_term_term xi_term) (upRen_term_term zeta_term)
            (upExtRen_term_term _ _ Eq_term) s1)
-  | tPair s0 s1 s2 s3 =>
-      congr_tPair (extRen_term xi_term zeta_term Eq_term s0)
-        (extRen_term (upRen_term_term xi_term) (upRen_term_term zeta_term)
-           (upExtRen_term_term _ _ Eq_term) s1)
+  | tPair s0 s1 s2 =>
+      congr_tPair
+        (option_ext
+           (extRen_term (upRen_term_term xi_term) (upRen_term_term zeta_term)
+              (upExtRen_term_term _ _ Eq_term)) s0)
+        (extRen_term xi_term zeta_term Eq_term s1)
         (extRen_term xi_term zeta_term Eq_term s2)
-        (extRen_term xi_term zeta_term Eq_term s3)
   | tFst s0 => congr_tFst (extRen_term xi_term zeta_term Eq_term s0)
   | tSnd s0 => congr_tSnd (extRen_term xi_term zeta_term Eq_term s0)
   end.
@@ -349,12 +348,13 @@ subst_term sigma_term s = subst_term tau_term s :=
       congr_tSig (ext_term sigma_term tau_term Eq_term s0)
         (ext_term (up_term_term sigma_term) (up_term_term tau_term)
            (upExt_term_term _ _ Eq_term) s1)
-  | tPair s0 s1 s2 s3 =>
-      congr_tPair (ext_term sigma_term tau_term Eq_term s0)
-        (ext_term (up_term_term sigma_term) (up_term_term tau_term)
-           (upExt_term_term _ _ Eq_term) s1)
+  | tPair s0 s1 s2 =>
+      congr_tPair
+        (option_ext
+           (ext_term (up_term_term sigma_term) (up_term_term tau_term)
+              (upExt_term_term _ _ Eq_term)) s0)
+        (ext_term sigma_term tau_term Eq_term s1)
         (ext_term sigma_term tau_term Eq_term s2)
-        (ext_term sigma_term tau_term Eq_term s3)
   | tFst s0 => congr_tFst (ext_term sigma_term tau_term Eq_term s0)
   | tSnd s0 => congr_tSnd (ext_term sigma_term tau_term Eq_term s0)
   end.
@@ -413,13 +413,14 @@ Fixpoint compRenRen_term (xi_term : nat -> nat) (zeta_term : nat -> nat)
         (compRenRen_term (upRen_term_term xi_term)
            (upRen_term_term zeta_term) (upRen_term_term rho_term)
            (up_ren_ren _ _ _ Eq_term) s1)
-  | tPair s0 s1 s2 s3 =>
-      congr_tPair (compRenRen_term xi_term zeta_term rho_term Eq_term s0)
-        (compRenRen_term (upRen_term_term xi_term)
-           (upRen_term_term zeta_term) (upRen_term_term rho_term)
-           (up_ren_ren _ _ _ Eq_term) s1)
+  | tPair s0 s1 s2 =>
+      congr_tPair
+        (option_comp
+           (compRenRen_term (upRen_term_term xi_term)
+              (upRen_term_term zeta_term) (upRen_term_term rho_term)
+              (up_ren_ren _ _ _ Eq_term)) s0)
+        (compRenRen_term xi_term zeta_term rho_term Eq_term s1)
         (compRenRen_term xi_term zeta_term rho_term Eq_term s2)
-        (compRenRen_term xi_term zeta_term rho_term Eq_term s3)
   | tFst s0 =>
       congr_tFst (compRenRen_term xi_term zeta_term rho_term Eq_term s0)
   | tSnd s0 =>
@@ -483,12 +484,14 @@ subst_term tau_term (ren_term xi_term s) = subst_term theta_term s :=
         (compRenSubst_term (upRen_term_term xi_term) (up_term_term tau_term)
            (up_term_term theta_term) (up_ren_subst_term_term _ _ _ Eq_term)
            s1)
-  | tPair s0 s1 s2 s3 =>
-      congr_tPair (compRenSubst_term xi_term tau_term theta_term Eq_term s0)
-        (compRenSubst_term (upRen_term_term xi_term) (up_term_term tau_term)
-           (up_term_term theta_term) (up_ren_subst_term_term _ _ _ Eq_term)
-           s1) (compRenSubst_term xi_term tau_term theta_term Eq_term s2)
-        (compRenSubst_term xi_term tau_term theta_term Eq_term s3)
+  | tPair s0 s1 s2 =>
+      congr_tPair
+        (option_comp
+           (compRenSubst_term (upRen_term_term xi_term)
+              (up_term_term tau_term) (up_term_term theta_term)
+              (up_ren_subst_term_term _ _ _ Eq_term)) s0)
+        (compRenSubst_term xi_term tau_term theta_term Eq_term s1)
+        (compRenSubst_term xi_term tau_term theta_term Eq_term s2)
   | tFst s0 =>
       congr_tFst (compRenSubst_term xi_term tau_term theta_term Eq_term s0)
   | tSnd s0 =>
@@ -568,14 +571,14 @@ ren_term zeta_term (subst_term sigma_term s) = subst_term theta_term s :=
         (compSubstRen_term (up_term_term sigma_term)
            (upRen_term_term zeta_term) (up_term_term theta_term)
            (up_subst_ren_term_term _ _ _ Eq_term) s1)
-  | tPair s0 s1 s2 s3 =>
+  | tPair s0 s1 s2 =>
       congr_tPair
-        (compSubstRen_term sigma_term zeta_term theta_term Eq_term s0)
-        (compSubstRen_term (up_term_term sigma_term)
-           (upRen_term_term zeta_term) (up_term_term theta_term)
-           (up_subst_ren_term_term _ _ _ Eq_term) s1)
+        (option_comp
+           (compSubstRen_term (up_term_term sigma_term)
+              (upRen_term_term zeta_term) (up_term_term theta_term)
+              (up_subst_ren_term_term _ _ _ Eq_term)) s0)
+        (compSubstRen_term sigma_term zeta_term theta_term Eq_term s1)
         (compSubstRen_term sigma_term zeta_term theta_term Eq_term s2)
-        (compSubstRen_term sigma_term zeta_term theta_term Eq_term s3)
   | tFst s0 =>
       congr_tFst
         (compSubstRen_term sigma_term zeta_term theta_term Eq_term s0)
@@ -659,14 +662,14 @@ subst_term tau_term (subst_term sigma_term s) = subst_term theta_term s :=
         (compSubstSubst_term (up_term_term sigma_term)
            (up_term_term tau_term) (up_term_term theta_term)
            (up_subst_subst_term_term _ _ _ Eq_term) s1)
-  | tPair s0 s1 s2 s3 =>
+  | tPair s0 s1 s2 =>
       congr_tPair
-        (compSubstSubst_term sigma_term tau_term theta_term Eq_term s0)
-        (compSubstSubst_term (up_term_term sigma_term)
-           (up_term_term tau_term) (up_term_term theta_term)
-           (up_subst_subst_term_term _ _ _ Eq_term) s1)
+        (option_comp
+           (compSubstSubst_term (up_term_term sigma_term)
+              (up_term_term tau_term) (up_term_term theta_term)
+              (up_subst_subst_term_term _ _ _ Eq_term)) s0)
+        (compSubstSubst_term sigma_term tau_term theta_term Eq_term s1)
         (compSubstSubst_term sigma_term tau_term theta_term Eq_term s2)
-        (compSubstSubst_term sigma_term tau_term theta_term Eq_term s3)
   | tFst s0 =>
       congr_tFst
         (compSubstSubst_term sigma_term tau_term theta_term Eq_term s0)
@@ -791,12 +794,13 @@ Fixpoint rinst_inst_term (xi_term : nat -> nat) (sigma_term : nat -> term)
       congr_tSig (rinst_inst_term xi_term sigma_term Eq_term s0)
         (rinst_inst_term (upRen_term_term xi_term) (up_term_term sigma_term)
            (rinstInst_up_term_term _ _ Eq_term) s1)
-  | tPair s0 s1 s2 s3 =>
-      congr_tPair (rinst_inst_term xi_term sigma_term Eq_term s0)
-        (rinst_inst_term (upRen_term_term xi_term) (up_term_term sigma_term)
-           (rinstInst_up_term_term _ _ Eq_term) s1)
+  | tPair s0 s1 s2 =>
+      congr_tPair
+        (option_ext
+           (rinst_inst_term (upRen_term_term xi_term)
+              (up_term_term sigma_term) (rinstInst_up_term_term _ _ Eq_term))
+           s0) (rinst_inst_term xi_term sigma_term Eq_term s1)
         (rinst_inst_term xi_term sigma_term Eq_term s2)
-        (rinst_inst_term xi_term sigma_term Eq_term s3)
   | tFst s0 => congr_tFst (rinst_inst_term xi_term sigma_term Eq_term s0)
   | tSnd s0 => congr_tSnd (rinst_inst_term xi_term sigma_term Eq_term s0)
   end.
